src/mqtt-packet-parser/src/main.fst
@@ -19,6 +19,8 @@ open Connect
 open Disconnect
 open Debug
 
+#set-options "--z3rlimit 10"
+
 val mqtt_packet_parse (packet_data: B.buffer U8.t) (packet_size: type_packet_size):
   Stack struct_fixed_header
     (requires (fun h ->
